src/riscv/Platform/MaterializeRiscvProgram.v
@@ -1,0 +1,80 @@
+Require Import riscv.Utility.Monads.
+Require Import riscv.Utility.FreeMonad.
+Require Import riscv.Spec.Decode.
+Require Import riscv.Spec.Machine.
+Require Import riscv.Utility.MkMachineWidth.
+Require Import riscv.Utility.Utility.
+
+Section Riscv.
+  Import free.
+  Context {W: Words}.
+
+  Variant action :=
+  | getRegister (_ : Register)
+  | setRegister (_ : Register) (_ : word)
+  | loadByte (_ : SourceType) (_ : word)
+  | loadHalf (_ : SourceType) (_ : word)
+  | loadWord (_ : SourceType) (_ : word)
+  | loadDouble (_ : SourceType) (_ : word)
+  | storeByte (_ : SourceType) (_ : word) (_ : w8)
+  | storeHalf (_ : SourceType) (_ : word) (_ : w16)
+  | storeWord (_ : SourceType) (_ : word) (_ : w32)
+  | storeDouble (_ : SourceType) (_ : word) (_ : w64)
+  | makeReservation (_ : word)
+  | clearReservation (_ : word)
+  | checkReservation (_ : word)
+  | getCSRField (_ : CSRField.CSRField)
+  | setCSRField (_ : CSRField.CSRField) (_ : MachineInt)
+  | getPrivMode
+  | setPrivMode (_ : PrivMode)
+  | endCycle (_ : Type)
+  | getPC
+  | setPC (_ : word)
+  | step
+  .
+
+  Definition result (action : action) : Type :=
+    match action with
+    | getRegister _ => word
+    | setRegister _ _ => unit
+    | loadByte _ _ => w8
+    | loadHalf _ _ => w16
+    | loadWord _ _ => w32
+    | loadDouble _ _ => w64
+    | storeByte _ _ _ | storeHalf _ _ _ | storeWord _ _ _ | storeDouble _ _ _ => unit
+    | makeReservation _ | clearReservation _ => unit
+    | checkReservation _ => bool
+    | getCSRField _ => MachineInt
+    | setCSRField _ _ => unit
+    | getPrivMode => PrivMode
+    | setPrivMode _ => unit
+    | endCycle T => T
+    | getPC => word
+    | setPC _ | step => unit
+    end.
+
+  Global Instance Materialize: RiscvProgram (free action result) word := {|
+    Machine.getRegister a := act (getRegister a) ret;
+    Machine.setRegister a b := act (setRegister a b) ret;
+    Machine.loadByte a b := act (loadByte a b) ret;
+    Machine.loadHalf a b := act (loadHalf a b) ret;
+    Machine.loadWord a b := act (loadWord a b) ret;
+    Machine.loadDouble a b := act (loadDouble a b) ret;
+    Machine.storeByte a b c := act (storeByte a b c) ret;
+    Machine.storeHalf a b c := act (storeHalf a b c) ret;
+    Machine.storeWord a b c := act (storeWord a b c) ret;
+    Machine.storeDouble a b c := act (storeDouble a b c) ret;
+    Machine.makeReservation a := act (makeReservation a) ret;
+    Machine.clearReservation a := act (clearReservation a) ret;
+    Machine.checkReservation a := act (checkReservation a) ret;
+    Machine.getCSRField f := act (getCSRField f) ret;
+    Machine.setCSRField f v := act (setCSRField f v) ret;
+    Machine.getPrivMode := act getPrivMode ret;
+    Machine.setPrivMode m := act (setPrivMode m) ret;
+    Machine.getPC := act getPC ret;
+    Machine.setPC a := act (setPC a) ret;
+    Machine.step := act step ret;
+    Machine.endCycle A := act (endCycle A) ret;
+  |}.
+
+End Riscv.
